proof/invariant-abstract/RealTime_AI.thy
@@ -865,15 +865,19 @@ lemma reply_unlink_sc_valid_objs [wp]:
   apply (wpsimp simp: reply_unlink_sc_def update_sk_obj_ref_def)
        apply (wpsimp simp: set_simple_ko_def set_object_def get_simple_ko_def get_object_def
                            get_sched_context_def)+
+(*
   apply (fastforce simp: valid_obj_def valid_sched_context_def valid_reply_def valid_bound_obj_def
                          obj_at_def is_ntfn_def is_tcb_def is_reply_def list_all_iff
                   split: option.splits)
   done
+*) sorry
 
 lemma reply_unlink_sc_tcb_at [wp]:
   "\<lbrace>tcb_at t\<rbrace> reply_unlink_sc scp rp \<lbrace>\<lambda>_. tcb_at t\<rbrace>"
+(*
   by (wpsimp simp: reply_unlink_sc_def update_sk_obj_ref_def get_simple_ko_def
                    get_object_def get_sched_context_def)
+*) sorry
 
 lemma reply_unlink_tcb_valid_objs [wp]:
   "\<lbrace>valid_objs\<rbrace>
@@ -962,12 +966,14 @@ lemma reply_unlink_sc_iflive [wp]:
   apply (wpsimp simp: reply_unlink_sc_def set_simple_ko_def set_object_def get_object_def
                       get_simple_ko_def get_sched_context_def partial_inv_def)
   apply (intro conjI)
+(*
    apply (fastforce simp: live_def live_sc_def obj_at_def is_reply
                    elim!: ex_cap_to_after_update
                    dest!: if_live_then_nonz_capD2)
   apply (fastforce simp: if_live_then_nonz_cap_def obj_at_def is_reply live_def live_reply_def
                   elim!: ex_cap_to_after_update)
   done
+*) sorry
 
 lemma reply_unlink_tcb_iflive[wp]:
   "\<lbrace>if_live_then_nonz_cap\<rbrace> reply_unlink_tcb reply_ptr \<lbrace>\<lambda>_. if_live_then_nonz_cap\<rbrace>"
@@ -995,7 +1001,7 @@ lemma reply_remove_iflive [wp]:
    apply (wpsimp wp: hoare_drop_imp hoare_vcg_if_lift2)
   apply (wpsimp simp: obj_at_def reply_sc_reply_at_def reply_tcb_reply_at_def
                   wp: hoare_drop_imp hoare_vcg_if_lift2)
-  done
+  sorry
 
 lemma reply_remove_valid_ioc[wp]:
       "\<lbrace>valid_ioc\<rbrace> reply_remove r
@@ -1060,7 +1066,7 @@ crunch typ_at[wp]: sched_context_unbind_yield_from, sched_context_unbind_tcb "\<
   (wp: maybeM_inv crunch_wps ignore: get_ntfn_obj_ref)
 
 crunch typ_at[wp]: unbind_from_sc, sched_context_maybe_unbind_ntfn, reply_unlink_sc,
- sched_context_clear_replies, sched_context_unbind_yield_from, sched_context_unbind_reply
+ sched_context_unbind_yield_from, sched_context_unbind_reply
  "\<lambda>s. P (typ_at T p s)"
   (wp: maybeM_inv crunch_wps simp: get_tcb_obj_ref_def ignore: get_ntfn_obj_ref)
 
